metaprog/custom_tactics.mli
@@ -17,6 +17,9 @@ module PVMonad : sig
   val ( let* ) : 'a Proofview.tactic -> ('a -> 'b Proofview.tactic) -> 'b Proofview.tactic
 end
 
+(** A direction in which to rewrite (using an equality). *)
+type rewrite_direction = LeftToRight | RightToLeft
+
 (** [intro_n n] introduces [n] variables/hypotheses with fresh names, but does not return
     the generated names to the caller. *)
 val intro_n : int -> unit Proofview.tactic
@@ -28,12 +31,11 @@ val intro_n : int -> unit Proofview.tactic
 val intro_fresh : string -> Names.Id.t Proofview.tactic
 
 (** [intro_rewrite dir] introduces a single equality and rewrites with it. [dir] controls
-    whether to rewrite left-to-right (if [true]) or right-to-left (if [false]). Default is
-    left-to-right. *)
-val intro_rewrite : dir:bool -> unit Proofview.tactic
+    in which direction to rewrite. *)
+val intro_rewrite : rewrite_direction -> unit Proofview.tactic
 
-(** [print_open_goals] prints a debug representation of each open goal. *)
-val print_open_goals : unit Proofview.tactic
+(** [print_open_goals ()] prints a debug representation of each open goal. *)
+val print_open_goals : unit -> unit Proofview.tactic
 
 (** [dispatch tac] applies [tac i] to the [i-th] open goal (starting at [0]). *)
 val dispatch : (int -> unit Proofview.tactic) -> unit Proofview.tactic
@@ -45,14 +47,19 @@ val dispatch : (int -> unit Proofview.tactic) -> unit Proofview.tactic
 val auto : ?depth:int -> ?lemmas:EConstr.t list -> unit -> unit Proofview.tactic
 
 (** [rewrite dir eq] rewrites with equality [eq], which can be a global constant or a
-    local variable. [dir] controls whether to rewrite left-to-right (if [true]) or
-    right-to-left (if [false]). Default is left-to-right.
+    local variable. [dir] controls in which direction to rewrite.
 
     Under the hood it uses [setoid_rewrite] (instead of [rewrite_strat]). *)
-val rewrite : dir:bool -> Names.GlobRef.t -> unit Proofview.tactic
+val rewrite : rewrite_direction -> Names.GlobRef.t -> unit Proofview.tactic
 
 (** [repeat_n n tac] applies [tac] exactly [n] times and returns the list of results. *)
 val repeat_n : int -> 'a Proofview.tactic -> 'a list Proofview.tactic
 
 (** [pattern t] abstracts the conclusion over all occurences of [t]. *)
 val pattern : EConstr.t -> unit Proofview.tactic
+
+(** [induction t] performs induction over [t]. *)
+val induction : EConstr.t -> unit Proofview.tactic
+
+(** [destruct t] destruct [t]. *)
+val destruct : EConstr.t -> unit Proofview.tactic
