plugin/main.ml
@@ -6,12 +6,13 @@ let main () =
     { n_ctors = 2
     ; base_types = [| EConstr.to_constr Evd.empty @@ Lazy.force Consts.string |]
     ; ctor_names = [| "App"; "Lam" |]
-    ; ctor_types = [| [ AT_term; AT_term ]; [ AT_base 0; AT_bind AT_term ] |]
+    ; ctor_types = [| [ AT_term; AT_term ]; [ AT_base 0; AT_bind (AT_bind AT_term) ] |]
     }
   in
   let ops0 = Gen_operations.generate s in
   let congr = Gen_congr_lemmas.generate s ops0 in
   let ops1 = Gen_signature.generate s ops0 in
   let re = Gen_reify_eval.generate s ops0 ops1 in
-  let _ = Gen_bijection.generate s ops0 ops1 congr re in
+  let bij = Gen_bijection.generate s ops0 ops1 congr re in
+  let _ = Gen_push_eval.generate s ops0 ops1 congr re bij in
   ()
