theories/Test.v
@@ -45,6 +45,38 @@ Print eval_ctor.
 Print eval.*)
 
 (*About eval_reify_inv.
-About seval_sreify_inv.*)
+About seval_sreify_inv.
+About term_ind'.*)
 
-About term_ind'.
+About eval_rename.
+About seval_rscomp.
+About seval_srcomp.
+About seval_scons.
+About seval_up_subst.
+
+Lemma eval_substitute (s : T.O.subst) (t : T.O.expr Kt) : 
+  eval Kt (T.O.substitute s t) = substitute (seval s) (eval Kt t).
+Proof.
+revert s. pattern t. apply term_ind' ; clear t.
+- intros i s. reflexivity.
+- intros t1 IH1 t2 IH2 s. repeat (simp substitute ; simpl). 
+  apply congr_App.
+  + rewrite IH1. reflexivity.
+  + rewrite IH2. reflexivity. 
+- intros str t IH s. repeat (simp substitute ; simpl). 
+  apply congr_Lam.
+  + reflexivity.
+  + rewrite IH. apply congr_substitute ; [|reflexivity].
+    repeat (rewrite seval_up_subst ; apply congr_up_subst).
+    reflexivity.
+Qed.
+
+
+(*Lemma eval_rename (r : ren) (t : T.O.expr Kt) :
+  eval Kt (T.O.rename r t) = rename r (eval Kt t).
+Proof.
+revert r. pattern t. apply term_ind'.
+- intros i r. reflexivity.
+- intros t1 IH1 t2 IH2 r. apply congr_App ; auto. 
+- intros str t1 IH1 r. apply congr_Lam ; auto. 
+Qed.*)
