README.md
@@ -1,0 +1,16 @@
+# Building 
+
+Create a local opam switch with the required packages:
+```
+opam switch create . 4.14.2 --repos=default,coq-released='https://coq.inria.fir/opam/released' -y
+```
+
+Optionally, install development packages, e.g. for VS Code:
+```
+opam install ocaml-lsp-server user-setup ocamlformat vscoq-language-server
+```
+
+Build with (`dune install` is required to step through Rocq files in VS Code):
+```
+dune build && dune install
+```
